ready to start chapter 3

src/natree/natree.lean
@@ -10,9 +10,8 @@ namespace natree
   def node : 𝕋 := ⟦▢⟧
   notation `△` := node
 
-  def app' (t₁ t₂) := ⟦t₁ ◦ t₂⟧
-  lemma app'_liftable {a₁ a₂ b₁ b₂} (h₁ : a₁ ≈ b₁) (h₂ : a₂ ≈ b₂) : app' a₁ a₂ = app' b₁ b₂ :=
-  begin
+  def app' : 𝕋' → 𝕋' → 𝕋 := λ t₁ t₂, ⟦t₁ ◦ t₂⟧
+  lemma app'_liftable {a₁ a₂ b₁ b₂} (h₁ : a₁ ≈ b₁) (h₂ : a₂ ≈ b₂) : app' a₁ a₂ = app' b₁ b₂ := begin
     repeat {rw wrapp},
     apply quotient.sound,
     apply pre.equiv.congr,
@@ -24,8 +23,7 @@ namespace natree
 
   theorem quot_dist_app {a b} : ⟦a ◦ b⟧ = ⟦a⟧ ⬝ ⟦b⟧ := rfl
 
-  theorem kernel {y z} : △⬝△⬝y⬝z = y :=
-  begin
+  theorem kernel {y z} : △⬝△⬝y⬝z = y := begin
     have h₁ := quotient.exists_rep y, cases h₁ with y' h₁, rw ←h₁,
     have h₂ := quotient.exists_rep z, cases h₂ with z' h₂, rw ←h₂,
     rw node,
@@ -34,8 +32,7 @@ namespace natree
     apply pre.equiv.kernel,
   end
 
-  theorem stem {x y z} : △⬝(△⬝x)⬝y⬝z = y⬝z⬝(x⬝z) :=
-  begin
+  theorem stem {x y z} : △⬝(△⬝x)⬝y⬝z = y⬝z⬝(x⬝z) := begin
     have h₁ := quotient.exists_rep x, cases h₁ with x' h₁, rw ←h₁,
     have h₂ := quotient.exists_rep y, cases h₂ with y' h₂, rw ←h₂,
     have h₃ := quotient.exists_rep z, cases h₃ with z' h₃, rw ←h₃,
@@ -45,8 +42,7 @@ namespace natree
     apply pre.equiv.stem,
   end
 
-  theorem fork {w x y z} : △⬝(△⬝w⬝x)⬝y⬝z = z⬝w⬝x :=
-  begin
+  theorem fork {w x y z} : △⬝(△⬝w⬝x)⬝y⬝z = z⬝w⬝x := begin
     have h₁ := quotient.exists_rep w, cases h₁ with w' h₁, rw ←h₁,
     have h₂ := quotient.exists_rep x, cases h₂ with x' h₂, rw ←h₂,
     have h₃ := quotient.exists_rep y, cases h₃ with y' h₃, rw ←h₃,
